test/test.qasm
@@ -6,6 +6,6 @@ creg c[2];
 
 id q[0];
 h q[0];
-id q[0];
+if(c == 0) id q[0];
 cx q[0], q[1];
 measure q[1] -> c[0];
